coq/JsInit.v
@@ -62,8 +62,8 @@ Notation "'attrib_native'" := prop_attributes_for_global_object.
 (** Builds an object with all optional fields to None
     and with extensible set to true *)
 
-Definition object_create_builtin vproto sclass builtinget P :=
-  object_create vproto sclass true builtinget P.
+Definition object_create_builtin vproto sclass P :=
+  object_create vproto sclass true P.
 
 (** Builds a native object, with [builtin_function_proto]
     as prototype, and a length property. *)
@@ -72,7 +72,7 @@ Definition object_create_builtin_common length P :=
   let sclass := "Function" in
   let P' := Heap.write P "length" (attrib_constant length) in
   (* The spec does not say anything special about [[get]] for built-in objects *)
-  object_create_builtin builtin_function_proto sclass builtin_spec_op_function_get P'.
+  object_create_builtin builtin_function_proto sclass P'.
 
 (** Builds a native function object, like in the above function
     but with only a Call method implemented by builtin code. *)
@@ -139,7 +139,6 @@ Definition object_builtin_global :=
   object_create_builtin
     object_builtin_global_proto
     object_builtin_global_class
-    builtin_spec_op_object_get
     object_builtin_global_properties.
 
 (**************************************************************)
@@ -166,7 +165,7 @@ Definition object_builtin_object_proto :=
   let P := write_native P "isPrototypeOf" builtin_object_proto_is_prototype_of in
   let P := write_native P "toString" builtin_object_proto_to_string in  
   let P := write_native P "valueOf" builtin_object_proto_value_of in 
-  object_create_builtin null "Object" builtin_spec_op_object_get P.
+  object_create_builtin null "Object" P.
 
 
 (**************************************************************)
@@ -187,7 +186,7 @@ Definition object_builtin_function_proto :=
   let P := Heap.empty in
   (* let P := write_native P "toString" builtin_function_proto_to_string in *) (* TODO *)
   (* LATER: complete list *)
-  object_create_builtin builtin_object_proto "Function" builtin_spec_op_object_get P.
+  object_create_builtin builtin_object_proto "Function" P.
 
 
 (**************************************************************)
@@ -212,7 +211,7 @@ Definition object_builtin_number_proto :=
   let P := write_native P "valueOf" builtin_number_proto_value_of in
   (* TODO: complete list *)
 
-  object_create_builtin builtin_object_proto "Number" builtin_spec_op_object_get P.
+  object_create_builtin builtin_object_proto "Number" P.
 
 
 (**************************************************************)
@@ -253,7 +252,7 @@ Definition object_builtin_bool_proto :=
   let P := write_native P "toString" builtin_bool_proto_to_string in   
   let P := write_native P "valueOf" builtin_bool_proto_value_of in
   (* TODO: complete list *)
-  object_create_builtin builtin_object_proto "Boolean" builtin_spec_op_object_get P. 
+  object_create_builtin builtin_object_proto "Boolean" P. 
 
 
 (**************************************************************)
